src/CCLHashExec.v
@@ -2,36 +2,25 @@ Require Import CCLProg.
 Require Import Hashmap.
 Require Import Automation.
 
-Local Lemma hm_upd : forall sigma up, Sigma.hm (Sigma.upd_disk sigma up) = Sigma.hm sigma.
-Proof.
-  destruct sigma; reflexivity.
-Qed.
-
 Theorem exec_hashmap_le : forall T (p: cprog T)
-                            G tid d_i sigma out,
-    exec G tid (ExecState d_i sigma) p out ->
+                            G tid sigma out,
+    exec G tid sigma p out ->
     match out with
-    | Finished (ExecState d_i' sigma') _ => hashmap_le (Sigma.hm sigma) (Sigma.hm sigma')
+    | Finished sigma' _ => hashmap_le (Sigma.hm sigma) (Sigma.hm sigma')
     | Error => True
     end.
 Proof.
   intros.
-  match goal with
-  | [ H: exec _ _ ?st _ _ |- _ ] => remember st
-  end.
   generalize dependent sigma.
-  generalize dependent d_i.
-  induction H; intros; auto; subst;
-    repeat match goal with
-           | [ x := _ |- _ ] => subst x
-           | [ H: ExecState _ _ = ExecState _ _ |- _ ] =>
-             inversion H; subst; clear H
-           | [ |- hashmap_le (Sigma.hm _) (Sigma.hm _) ] =>
-             repeat match goal with
-                    | [ sigma: Sigma |- _ ] => destruct sigma
-                    end; simpl in *; reflexivity
-           end.
-  - destruct sigma0.
+  induction 1; intros; auto;
+      repeat match goal with
+             | [ x := _ |- _ ] => subst x
+             | [ |- hashmap_le (Sigma.hm _) (Sigma.hm _) ] =>
+               repeat match goal with
+                      | [ sigma: Sigma |- _ ] => destruct sigma
+                      end; simpl in *; reflexivity
+             end.
+  - destruct sigma.
     destruct p;
       repeat match goal with
              | [ H: context[match ?d with | _ => _ end] |- _ ] =>
@@ -40,7 +29,6 @@ Proof.
                inversion H; subst; clear H
              | [ |- hashmap_le ?a ?a ] => reflexivity
              | _ => progress simpl in *
-             | _ => progress rewrite hm_upd
              | _ => congruence
              end.
   - repeat match goal with
@@ -53,19 +41,11 @@ Proof.
     econstructor; eauto.
     constructor.
   - destruct out; eauto.
-    specialize (IHexec1 _ _ ltac:(eauto)).
-    destruct st'.
-    specialize (IHexec2 _ _ ltac:(eauto)).
-    destruct sigma0.
     etransitivity; eauto.
   - destruct sigma'; simpl in *.
     eauto.
-  - inversion H0; subst; eauto.
-    destruct sigma0; reflexivity.
-  - destruct (Sigma.l sigma0); intuition eauto.
-    subst; reflexivity.
-  - inversion H1; subst; eauto.
-    destruct sigma0; reflexivity.
+  - destruct (Sigma.l sigma); intuition subst.
+    reflexivity.
 Qed.
 
 (* Local Variables: *)
